Weidenbach_Book/Watched_Literals_Algorithm_Restart.thy
@@ -482,7 +482,7 @@ lemma cdcl_twl_stgy_restart_with_leftovers_refl: \<open>cdcl_twl_stgy_restart_wi
   by (rule exI[of _ \<open>fst S\<close>]) auto
 
 (* declare restart_prog_spec[THEN order_trans, refine_vcg] *)
-lemma (in twl_restart) cdcl_twl_stgy_prog_spec:
+lemma (in twl_restart) cdcl_twl_stgy_restart_prog_spec:
   assumes \<open>twl_struct_invs S\<close> and \<open>twl_stgy_invs S\<close> and \<open>clauses_to_update S = {#}\<close> and
     \<open>get_conflict S = None\<close>
   shows
